
\begin{longfbox}
      \begin{bt} \label{pro:practice1.5}
            Các tập được xét đến đều là tập con của một tập vũ trụ $\mathcal U$ nào đó. Hãy kiểm tra các đẳng thức tập hợp sau đây
      \end{bt}
\end{longfbox}

Solution:
\begin{enumerate}
\item[a)] $A\cap (A^\mathsf{c}\cup B\cup C) = (A\cap B)\cup(A\cap C)$ \\
      \begin{align}
            A\cap (A^\mathsf{c}\cup B\cup C)
            &= (A\cap A^\mathsf{c})\cup (A\cap(B\cup C)) \\
            &= \emptyset\cup(A\cap(B\cup C)) \\
            &= A\cap(B\cup C) \\
            &= (A\cap B)\cup(A\cap C)
      \end{align} 
      So, proved!
\item[b)] $(A\cap B\cap C^\mathsf{c})\cup(A\cap B^\mathsf{c}\cap C) = A\cap (B\bigtriangleup C)$ \\
      \begin{align}
            A\cap (B\bigtriangleup C)
            &= A\cap((B\setminus C)\cup(C\setminus B)) \\
            &= A\cap((B\cap C^\mathsf{c})\cup(C\cap B^\mathsf{c})) \\
            &= (A\cap B\cap C^\mathsf{c})\cup(A\cap B^\mathsf{c}\cap C)
      \end{align} 
      So, proved!
\item[c)] $(A\cap B\cap C^\mathsf{c})\cup(A\cap B^\mathsf{c}\cap C^\mathsf{c}) = A\cap C^\mathsf{c}$ \\
      \begin{align}
            (A\cap B\cap C^\mathsf{c})\cup(A\cap B^\mathsf{c}\cap C^\mathsf{c})
            &= (A\cap C^\mathsf{c}\cap B)\cup(A\cap C^\mathsf{c}\cap B^\mathsf{c}) \\
            &= A\cap C^\mathsf{c}\cap(B\cup B^\mathsf{c}) \\
            &= A\cap C^\mathsf{c}\cap\mathcal U \\
            &= A\cap C^\mathsf{c}
      \end{align} 
      So, proved!
\item[d)] $(A\cap(B\cap C)^\mathsf{c}) = (A\cap B^\mathsf{c})\cup(A\cap C^\mathsf{c})$ \\
      \begin{align}
            (A\cap(B\cap C)^\mathsf{c})
            &= A\cap(B^\mathsf{c}\cup C^\mathsf{c}) \\
            &= (A\cap B^\mathsf{c})\cup(A\cap C^\mathsf{c})
      \end{align} 
      So, proved!
\item[e)] $(A\cup(B\cap C)^\mathsf{c}) = (A\cup B^\mathsf{c})\cup(A\cup C^\mathsf{c})$ \\
      \begin{align}
            (A\cup(B\cap C)^\mathsf{c})
            &= A\cup(B^\mathsf{c}\cup C^\mathsf{c}) \\
            &= A\cup B^\mathsf{c}\cup C^\mathsf{c} \\
            &= A\cup A\cup B^\mathsf{c}\cup C^\mathsf{c} \\
            &= A\cup B^\mathsf{c}\cup A\cup C^\mathsf{c} \\
            &= (A\cup B^\mathsf{c})\cup (A\cup C^\mathsf{c})
      \end{align} 
      So, proved!
\end{enumerate}